cleaning

VmSemantics.v
@@ -145,13 +145,11 @@ Inductive vm_step' : vm_config -> vm_config -> list Ev -> Prop  :=
     vm_step' (mk_vm_config e ([i] ++ l) s) (mk_vm_config e' l s') tr.
 
 Definition vm_1n_multi : step_relation vm_config Ev := refl_trans_1n_trace vm_step'.
-Check vm_1n_multi.
 
 Definition vm_1n_multi' (acc1:vm_accum) (acc2:vm_accum) (el_in:list AnnoInstr) (el_out:list AnnoInstr) (tr:list Ev) :=
   vm_1n_multi (mk_vm_config (ec acc1) el_in (vm_stack acc1))
               (mk_vm_config (ec acc2) el_out (vm_stack acc2))
               tr.
-Check vm_1n_multi'.
 
 Lemma vm_1n_multi_trans : forall x y z tr tr',
   vm_1n_multi x y tr ->
@@ -160,39 +158,6 @@ Lemma vm_1n_multi_trans : forall x y z tr tr',
 Proof.
   apply refl_trans_1n_trace_trans.
 Defined.
-
-Check refl_trans_1n_trace_trans.
-
-(*
-Lemma fafa : forall r r' tr i rest,
-    vm_step' r i r' tr ->
-    vm_lstar r r' ([i] ++ rest) rest tr.
-      
-Inductive vm_lstar: vm_accum -> vm_accum -> list AnnoInstr -> list AnnoInstr -> list Ev -> Prop :=
-| vm_lstar_refl: forall r, vm_lstar r r [] [] []
-| vm_lstar_tran: forall i l l' r r' r'' tr1 tr2,
-    vm_step r i r' tr1 -> vm_lstar r' r'' l l' tr2 -> vm_lstar r r'' (i::l) l' (tr1 ++ tr2).
-Hint Resolve vm_lstar_refl. *)
-
-(*
-Lemma vm_lstar_trans : forall r r' r'' il il' il'' tr1 tr2,
-  vm_lstar r r' il il' tr1 ->
-  vm_lstar r' r'' il' il'' tr2 ->
-  vm_lstar r r'' il il'' (tr1 ++ tr2).
-Proof.
-  intros.
-  generalize dependent r''.
-  generalize dependent il''.
-  induction H; intros.
-  - inv H0. econstructor.
-    (*simpl.
-    econstructor; eauto.*)
-  - rewrite <- app_assoc.
-    eapply vm_lstar_tran.
-    apply H.
-    eauto.
-Defined. *)
-
 
 Lemma ha : forall r r' r'' il1 il2 resl tr1 tr2,
   vm_1n_multi' r r' (il1 ++ il2) il2 tr1 ->
@@ -215,7 +180,6 @@ Proof.
   generalize dependent resl.
   generalize dependent tr2.
   generalize dependent il2.
-  (*eapply vm_1n_multi_trans; eauto.*)
   dependent induction H; intros.
   - eauto.
   - inv H.
@@ -228,7 +192,6 @@ Proof.
     eapply IHrefl_trans_1n_trace; eauto.
 Defined.
 
-
 Lemma vm_1n_multi_transitive: 
   forall r r' r'' il1 il2 resl tr1 tr2,
     vm_1n_multi' r r' il1 [] tr1 ->
@@ -240,16 +203,6 @@ Proof.
   eapply vm_1n_multi_transitive'; eauto.
 Defined.
 
-(*
-Lemma vm_1n_multi_transitive': forall e e' e'' s s' s'' il1 il2 tr1 tr2 resl,
-    vm_1n_multi (mk_vm_config e il1 s) (mk_vm_config e' [] s') tr1 ->
-    vm_1n_multi (mk_vm_config e' il2 s') (mk_vm_config e'' resl s'') tr2 ->
-    vm_1n_multi (mk_vm_config e (il1 ++ il2) s) (mk_vm_config e'' resl s'') (tr1 ++ tr2).
-Proof.*)
-
-  
-
-
 Lemma vm_1n_multi_transitive_done: forall r r' r'' il1 il2 tr1 tr2,
     vm_1n_multi' r r' il1 [] tr1 ->
     vm_1n_multi' r' r'' il2 [] tr2 ->
@@ -258,8 +211,6 @@ Proof.
   intros.
   eapply vm_1n_multi_transitive; eauto.
 Defined.
-
-  
 
 Lemma vm_1n_multi_transitive_done': forall e e' e'' s s' s'' il1 il2 tr1 tr2,
     vm_1n_multi (mk_vm_config e il1 s) (mk_vm_config e' [] s') tr1 ->
@@ -271,14 +222,6 @@ Proof.
 Defined.
 
 Definition vm_n1_multi : step_relation vm_config Ev := refl_trans_n1_trace vm_step'.
-
-    (*
-Inductive vm_rlstar: vm_accum -> vm_accum -> list AnnoInstr -> list AnnoInstr -> list Ev -> Prop :=
-| vm_rlstar_refl: forall r, vm_rlstar r r [] [] []
-| vm_rlstar_tran: forall r r' r'' i il tr1 tr2,
-    vm_rlstar r r' il [] tr1 -> vm_step r' i r'' tr2 ->
-    vm_rlstar r r'' (il ++ [i]) [] (tr1 ++ tr2).
-Hint Resolve vm_rlstar_refl. *)
 
 Lemma vm_n1_implies_1n : forall r r' tr,
     vm_n1_multi r r' tr -> vm_1n_multi r r' tr.
@@ -326,6 +269,107 @@ Proof.
   rewrite <- vm_n1_iff_1n; eauto.
 Defined.
 
+Lemma step_implies_lstar : forall e e' s s' i tr,
+    vm_step (mk_accum e s) i (mk_accum e' s') tr ->
+    vm_1n_multi (mk_vm_config e [i] s) (mk_vm_config e' [] s') tr.
+Proof.
+  intros.
+  cut ( vm_1n_multi {| cec := e; cvm_list := ([i] ++ []); cvm_stack := s |}
+                    {| cec := e'; cvm_list := []; cvm_stack := s' |} (tr ++ [])). simpl. rewrite app_nil_r. eauto.
+  repeat econstructor; eauto.
+Defined.
+
+Lemma record_congr : forall r,
+  r = 
+  {| ec := ec r; vm_stack := vm_stack r |}.
+Proof.
+  intros.
+  destruct r.
+  reflexivity.
+Defined.
+
+Lemma restt : forall r r' r'' il il1 tr1 tr2 i,
+  vm_n1_multi' r r' il [] tr1 ->
+  vm_step r' i r'' tr2 ->
+  il1 = il ++ [i] ->
+  vm_1n_multi' r r'' il1 [] (tr1 ++ tr2).
+Proof.
+  intros.
+  rewrite H1.
+  eapply vm_1n_multi_transitive'.
+  unfold vm_n1_multi' in H.
+  rewrite vm_n1_iff_1n in H.
+  eapply H.
+  apply step_implies_lstar.
+  cut (vm_step r' i r'' tr2). repeat rewrite <- record_congr. auto.
+  assumption.
+Defined.
+
+Fixpoint shave_r{A} (l: list A) : list A :=
+  match l with
+  | [] => []
+  | [x] => []
+  | x::l => x :: shave_r l
+  end.
+
+Lemma restl : forall r r' r'' il1 il2 i cs cs',
+    vm_1n_multi' r r' (il1 ++ il2) (i::il2) cs /\
+    vm_step r' i r'' cs' ->
+    vm_1n_multi' r r'' il1 [] (cs ++ cs').
+Proof.
+  intros.
+  destruct H.
+  eapply restt with (il:=shave_r il1).
+  unfold vm_1n_multi' in H.
+  rewrite <- vm_n1_iff_1n in H.
+  inv H.
+  admit.
+
+  dependent destruction x'.
+  inv H2.
+(*
+  assert (cvm_list0 = shave_r il1). admit. rewrite H in H1. rewrite H in H2.
+  unfold vm_n1_multi'.
+  eapply vm_n1_multi_transitive.
+  
+  apply H0.
+  intros.
+  destruct H.
+  generalize dependent cs'.
+ 
+  unfold vm_1n_multi' in H.
+  rewrite <- vm_n1_iff_1n in H.
+  dependent induction H; intros.
+  - 
+  assert (il1 = [i]). admit.
+  rewrite H.
+  eapply step_implies_lstar. simpl. repeat rewrite <- record_congr.
+  assert (r = r'). admit.
+  rewrite H1. auto.
+  -
+    rewrite <- app_assoc.
+
+    
+    (*assert (cs'0 = []). admit. rewrite H2. rewrite app_nil_r.*)
+    dependent destruction x'.
+    
+    eapply IHrefl_trans_n1_trace with (r':=(mk_accum e s)). reflexivity.
+    inversion H0. rewrite H5 in H3. rewrite H3.
+    reflexivity.
+    assert (cvm_list0 = i :: il2). admit.
+    assert (cec0 = ec r'). admit.
+    assert (cvm_stack0 = vm_stack r'). admit.
+    subst. reflexivity.
+    assumption.
+
+
+    congruence.
+    rewrite H3. reflexivity.
+    eassumption.
+ *)
+Admitted.
+
+
 (*
 Ltac inv_vm_lstar :=
   repeat (
@@ -334,46 +378,17 @@ Ltac inv_vm_lstar :=
       | [ G: vm_step _ _ _ _ |- _ ] => inv G; simpl
       end).  *)
 
-(*
-Lemma restl : forall r r' r'' il1 il2 i cs cs',
-    vm_1n_multi' r r' (il1 ++ il2) (i::il2) cs /\
-    vm_step r' i r'' cs' ->
-    vm_1n_multi' r r'' il1 [] (cs ++ cs').
-Proof.
-  intros.
-  destruct H.
-  inv H.
-  - assert (il1 = [i]).
-    admit.
-    rewrite H.
-    assert (r = r').
-    admit.
-    rewrite H1.
-    admit.
-  - dependent destruction x'.
-    inv H1.
-Admitted. *)
-
-(*   r, r', r'' : vm_accum
-  i : AnnoInstr
-  il : list AnnoInstr
-  tr1, tr2 : list Ev
-  H : vm_rlstar r r' il [] tr1
-  H0 : vm_step r' i r'' tr2
-  IHvm_rlstar : forall il1 : list AnnoInstr,
-                il = il1 ++ [] -> vm_lstar r r' il1 [] tr1
-  il1 : list AnnoInstr
-  x : il ++ [i] = il1 ++ []
-  ============================
-  vm_lstar r r'' il1 [] (tr1 ++ tr2) *)
-
 
 Lemma hh {A:Type}:
   forall (l1:list A) l2,
     l1 ++ l2 = l2 ->
     l1 = [].
 Proof.
-Admitted.
+  intros.
+  Search (_ ++ _ = _).
+  eapply app_inv_tail.
+  apply H.
+Defined.
 
 Lemma hhh : forall r',
     {| ec := ec r'; vm_stack := vm_stack r' |} = r'.
@@ -383,9 +398,6 @@ Proof.
   destruct r'.
   auto.
 Defined.
-
-
-
 
 Lemma fafa : forall e e' s s' tr i rest,
     vm_step (mk_accum e s) i (mk_accum e' s') tr ->
@@ -406,6 +418,39 @@ Lemma ffff_gen_helperrr : forall r r' il1 il1' il2 tr,
   vm_1n_multi' r r' il1 il1' tr ->
   vm_1n_multi' r r' (il1 ++ il2) (il1' ++ il2) tr.
 Proof.
+  intros.
+  inv H0.
+  - assert (r = r'). admit. rewrite H0.
+    econstructor.
+  - 
+    dependent destruction x'.
+    inv H1.
+    Lemma afaf : forall r r' i l' cs,
+        vm_step r i r' cs -> 
+    vm_step' (mk_vm_config (ec r) (i::l') (vm_stack r))
+             (mk_vm_config (ec r') l'     (vm_stack r'))
+             cs.
+    Proof.
+    Admitted.
+    assert ((i :: cvm_list0) ++ il2 = i :: (cvm_list0 ++ il2)). auto.
+    rewrite H0.
+    econstructor.
+
+    apply afaf.  rewrite <- record_congr in H9. apply H9. clear H0. clear H9.
+    (*
+    assert (cs' = [] ++ cs').(* rewrite app_nil_r.*) auto.
+
+    rewrite H0.
+    eapply vm_1n_multi_transitive.
+    econstructor.
+    
+  ============================
+  vm_step'
+    {|
+    cec := ec r;
+    cvm_list := (i :: cvm_list0) ++ il2;
+    inv H9
+    eapply vm_1n_multi_transitive' *)  
 Admitted.
 
 (*
@@ -449,6 +494,7 @@ Proof.
   eapply ffff_gen_helperrr; eauto.
 Defined. *)
 
+(*
 Lemma asdd {A:Type} : forall l (v:A) il1 il2,
     l ++ [v] = il1 ++ il2 ->
     (il2 = [] /\ l ++ [v] = il1) \/
@@ -456,7 +502,7 @@ Lemma asdd {A:Type} : forall l (v:A) il1 il2,
     (il2 = [v] /\ l = il1) \/
     (exists n, (il1 = firstn n l) /\ (il2 = (skipn n l) ++ [v])).
 Proof.
-Admitted.
+Admitted.*)
 
 Lemma list_nil_app{A:Type} : forall (l1 l2:list A),
     [] = l1 ++ l2 ->
@@ -469,15 +515,7 @@ Proof.
   - inv H.
 Defined. 
 
-Lemma step_implies_lstar : forall e e' s s' i tr,
-    vm_step (mk_accum e s) i (mk_accum e' s') tr ->
-    vm_1n_multi (mk_vm_config e [i] s) (mk_vm_config e' [] s') tr.
-Proof.
-  intros.
-  cut ( vm_1n_multi {| cec := e; cvm_list := ([i] ++ []); cvm_stack := s |}
-                    {| cec := e'; cvm_list := []; cvm_stack := s' |} (tr ++ [])). simpl. rewrite app_nil_r. eauto.
-  repeat econstructor; eauto.
-Defined.
+
 
 Lemma first_skip{A:Type} :
   forall n (l:list A),
@@ -485,6 +523,7 @@ Lemma first_skip{A:Type} :
 Proof.
 Admitted.
 
+(*
 Lemma ffff_another_helper :forall r r3 tr il1 il2 resl,
     il1 <> [] ->
     vm_1n_multi' r r3
@@ -498,7 +537,7 @@ Lemma ffff_another_helper :forall r r3 tr il1 il2 resl,
         vm_1n_multi' r' r3
                  il2 resl
                  tr2.
-Admitted.
+Admitted.*)
 
 
 
@@ -589,6 +628,7 @@ Proof.
 Defined.
 *)
 
+(*
 Lemma ffff_gen_helper :forall r r3 tr il1 il2,
     (il1 <> []) ->
   vm_1n_multi' r r3
@@ -605,7 +645,7 @@ Lemma ffff_gen_helper :forall r r3 tr il1 il2,
 Proof.
   intros.
   eapply ffff_another_helper; eauto.
-Defined.
+Defined. *)
 
 
 
@@ -630,7 +670,7 @@ Proof.
 Defined.
  *)
 
-
+(*
 Lemma ffff_gen_helper' : forall r r' il1 il2 tr,
   vm_1n_multi' r r' (il1 ++ il2) il2 tr ->
   vm_1n_multi' r r' il1 [] tr.
@@ -654,7 +694,7 @@ Proof. (*
     rewrite <- H.
     eauto.
 Defined.*)
-Admitted.
+Admitted. *)
 
 (*
 Lemma ffff_gen_helper' : forall r r' il1 il2 tr,
@@ -674,6 +714,7 @@ Proof.
     eapply vm_rlstar_tran; eauto.
 Defined. *)
 
+(*
 Lemma ffff_gen :forall r r3 tr il1 il2,
     il1 <> [] ->
     vm_1n_multi' r r3
@@ -723,7 +764,7 @@ Proof.
               {| ec := e'; vm_stack := s' |} {| ec := ec0; vm_stack := vm_stack0 |} (firstn H1 l) [] cs'). auto.
       eapply ffff_gen_helper'; eauto.
 Admitted.
-
+*)
 
 
 (*
@@ -751,6 +792,7 @@ Lemma compile_not_empty :
 Proof.
 Admitted.
 
+(*
 Lemma ffff : forall r t tr r3 il2, (* TODO: il1 must be compiled for stack restore *)
     let il1 := (instr_compiler t) in
     vm_1n_multi' r r3
@@ -772,6 +814,7 @@ Proof.
   apply compile_not_empty.
   eauto.
 Defined.
+*)
 
 Lemma lstar_stls :
   forall st0 st1 t tr,
@@ -829,62 +872,454 @@ Defined.
 Axiom para_eval_vm : forall t e,
     parallel_eval_thread (unanno t) e = parallel_att_vm_thread (instr_compiler t) e.
 
-(*
-Lemma ffff : forall r t tr r3 il2, (* TODO: il1 must be compiled for stack restore *)
-    let il1 := (instr_compiler t) in
-    vm_1n_multi' r r3
-             (il1 ++ il2) []
-             tr ->
-   exists r' tr1,
-      vm_1n_multi' r r'
-               il1 []
-               tr1 /\
-     exists tr2,
-       vm_1n_multi' r' r3
-               il2 []
-               tr2.
+Lemma jj : forall e e' s t rest tr,
+    vm_1n_multi
+      {| cec := e; cvm_list := instr_compiler t; cvm_stack := s |}
+      {| cec := e'; cvm_list := []; cvm_stack := s |} tr ->
+    
+    vm_1n_multi
+      {| cec := e;
+         cvm_list := instr_compiler t ++ rest ;
+         cvm_stack := s |}
+      {| cec := e';
+         cvm_list := rest;
+         cvm_stack := s |} tr.
 Proof.
   intros.
-  unfold vm_1n_multi' in H.
-  (*rewrite <- vm_n1_iff_1n in H.*)
-  dependent induction H.
-  - assert (il1 = [] /\ il2 = []).
-    admit.
-    destruct H. rewrite H.
-    eexists. eexists.
-    split.
-    econstructor.
-    rewrite H0.
-    eexists.
-    assert (r = r3).
-    admit.
-    rewrite H1.
-    econstructor.
-  - Check asdd.
-    eapply IHrefl_trans_1n_trace.
-    reflexivity.
-    edestruct IHrefl_trans_n1_trace. admit.
+  assert (rest = [] ++ rest). simpl. reflexivity.
+  rewrite H0 at 2.
+  assert (tr = tr ++ []). rewrite app_nil_r. auto.
+  rewrite H1.
+  eapply vm_1n_multi_transitive'. apply H.
+  simpl. econstructor.
+Defined.
+
+Axiom hihi : forall t tr,
+    trace t tr -> (parallel_vm_events (instr_compiler t) = tr).
+
+Axiom hihi' : forall t tr,
+    (parallel_vm_events (instr_compiler t) = tr) -> trace t tr.
+
+(*
+Lemma stack_restore_vm : forall e e' s s' t tr,
+    vm_lstar (mk_accum e s) (mk_accum e' s')
+             (instr_compiler t) [] tr ->
+    s = s'.
+Proof.
+  intros.
+  edestruct vm_config_correct; eauto.
+Defined.*)
 
 
+
+(*
+Lemma all_tt :
+  forall t r,
+  exists r' tr,
+    vm_1n_multi' r r'
+                   (instr_compiler t) [] tr (*/\ trace t tr*).
+Proof.
+Admitted.*)
+
+(*
+Lemma aa : forall r r' t1 t2 tr x y rg,
+    vm_1n_multi' r r'
+                 (instr_compiler (alseq rg t1 t2)) [] tr ->
+    trace t1 x ->
+    trace t2 y ->
+    tr = x ++ y.
+Proof.
+  intros.
+  inv H.
+  - admit.
+  - 
     
-    dependent destruction x'. doit.
-    eapply IHrefl_trans_n1_trace.
-    reflexivity. admit
-    edestruct IHrefl_trans_n1_trace.
-    reflexivity.
-    reflexivity.
     
+Admitted. *)
+
+(*
+Lemma tryit : forall r r' r'' t il2 tr1 tr,
+  vm_1n_multi' r r''
+               (instr_compiler t ++ il2)
+               []
+               tr
+  ->
+  vm_1n_multi' r r'
+               (instr_compiler t)
+               []
+               tr1
+  -> vm_1n_multi' r' r''
+                 il2
+                 []
+                 (skipn (length tr1) tr).
+Admitted. *)
+
+
+(*
+Definition instrEvent (ai:AnnoInstr) : list Ev :=
+  match ai with
+  | aprimInstr i pi => prim_trace i pi
+  | asplit i _ _ => [Term.split i]
+  | ajoins i => [Term.join i]
+  | ajoinp i => [Term.join i]
+  | abesr => []
+  | areqrpy r _ _ 
+  | _ => []
+  end.
+    
+Admitted.
+
+Inductive progDenote: list AnnoInstr -> list Ev -> Prop :=
+| doneden : progDenote [] []
+| iden: forall i, progDenote [i] (instrEvent i)
+| progden: forall x y el1 el2,
+    progDenote x el1 ->
+    progDenote y el2 ->
+    progDenote (x ++ y) (el1 ++ el2).
+
+
+Theorem heyit : forall t tr,
+    progDenote (instr_compiler t) tr -> trace t tr.
+Proof.
+  intros.
+  generalize dependent tr.
+  induction t; intros.
+  - admit.
+  - inv H.
+    
+    
+Admitted.
+
+
+Theorem intermed : forall t tr1 tr2 il2,
+  progDenote (instr_compiler t) tr1 ->
+  progDenote il2 tr2 ->
+  progDenote (instr_compiler t ++ il2) (tr1 ++ tr2).
+   *) 
+  
+  
+Lemma destr_app_compile : forall r0 r' t1 t2 tr r,
+    vm_1n_multi' r0 r' (instr_compiler (alseq r t1 t2)) [] tr
+    -> (exists tr1 r_mid,
+          vm_1n_multi' r0 r_mid (instr_compiler t1) [] tr1 /\
+          exists tr2,
+            vm_1n_multi' r_mid r' (instr_compiler t2) [] tr2 /\
+            tr = tr1 ++ tr2).
+Proof. (*
+  intros.
+  dependent induction t1.
+  admit.
+  apply IHn.*)
+
+
+(*
+  intros.
+  dependent destruction r0.
+  (*destruct all_t with (t:= t1) (e:=ec0) (s:=vm_stack0).*)
+  destruct_conjs.
+  assert (vm_1n_multi' {| ec := ec0; vm_stack := vm_stack0 |}
+                       {| ec := (eval (unanno t1) ec0); vm_stack := vm_stack0 |} (instr_compiler t1) [] x).
+  apply vm_config_correct. eauto.
     
   
+  exists x.
+  exists (mk_accum (eval (unanno t1) ec0) vm_stack0).
+
+  split.
+  eassumption. clear H2.
+  destruct all_t with (t:= t2) (e:=eval (unanno t1) ec0) (s:=vm_stack0).
+  destruct_conjs.
+
+  assert ( vm_1n_multi'
+             {| ec := (eval (unanno t1) ec0); vm_stack := vm_stack0 |}
+             {| ec := (eval (unanno t2) (eval (unanno t1) ec0)); vm_stack := vm_stack0 |}
+             (instr_compiler t2) []
+             x0).
+  apply vm_config_correct. eauto.
+
+  assert (tr = x ++ x0).
+
+  eapply aa; eauto.
+
+
+  
+  assert ( vm_1n_multi' {| ec := ec0; vm_stack := vm_stack0 |}
+                        {| ec := eval (unanno (alseq r t1 t2)) ec0; vm_stack := vm_stack0 |}
+                        
+                        (instr_compiler (alseq r t1 t2 )) [] tr).
+  
+  eapply vm_config_correct.
+  {
+  rewrite H9.
+  econstructor; eauto. }
+  exists x0.
+  
+  split.
+
+  assert (r' = {|
+         ec := eval (unanno t2) (eval (unanno t1) ec0);
+         vm_stack := vm_stack0 |}).
+  simpl in H8.
+  admit. (* TODO: vm_config_deterministic *)
+  subst.
+  eassumption.
+  eassumption. *)
 Admitted.
- *)
+
+Lemma destr_app_compile': forall r0 r' t1 t2 tr n,
+    vm_1n_multi' r0 r' (instr_compiler t1 ++
+                         abesr :: instr_compiler t2 ++ [ajoins n]) [] tr
+    -> (exists tr1 r_mid,
+          vm_1n_multi' r0 r_mid (instr_compiler t1) [] tr1 /\
+          exists tr2,
+            vm_1n_multi' r_mid r' (abesr :: instr_compiler t2 ++ [ajoins n]) [] tr2 /\
+            tr = tr1 ++ tr2).
+Proof.
+  intros.
+Admitted.
+
+Lemma destr_app_compile'': forall r0 r' t2 tr n,
+    vm_1n_multi' r0 r' (instr_compiler t2 ++ [ajoins n]) [] tr
+    -> (exists tr1 r_mid,
+          vm_1n_multi' r0 r_mid (instr_compiler t2) [] tr1 /\
+          exists tr2,
+            vm_1n_multi' r_mid r' ([ajoins n]) [] tr2 /\
+            tr = tr1 ++ tr2).
+Proof.
+Admitted.
+
+Lemma vm_lstar_trace: forall r r' t tr,
+    (*well_formed t -> *)
+    vm_1n_multi' r r'
+             (instr_compiler t) []
+             tr ->
+    trace t tr.
+Proof.
+  intros.
+  (*assert (tr <> []). admit.*)
+  generalize dependent r.
+  generalize dependent r'.
+  generalize dependent tr.
+  induction t; intros.
+  - destruct a; simpl.
+    + simpl.
+      inv H.
+      inv H1. inv H0. inv H7. simpl. econstructor. inv H0. inv H8. inv H.
+    + admit.
+    +
+      admit.
+    +
+      admit.
+    + admit.
+      (*
+      inv H2.
+      * simpl. econstructor.
+      * inv H.
+    + simpl.
+      inv H.
+      inv H1. inv H8.
+      inv H2.
+      * simpl. econstructor.
+      * inv H.
+    + simpl.
+      inv H.
+      inv H1. inv H8.
+      inv H2.
+      * simpl. econstructor.
+      * inv H.
+    + simpl.
+      inv H.
+      inv H1. inv H8.
+      inv H2.
+      * simpl. econstructor.
+      * inv H.
+    + simpl.
+      inv H.
+      inv H1. inv H8.
+      inv H2.
+      * simpl. econstructor.
+      * inv H. *)
+  - admit. (*inv H.
+    dependent destruction x'.
+    inv H1. inv H10.
+    inv H2.
+    simpl. rewrite app_nil_r.
+    
+    econstructor.
+    eapply IHt.
+    admit.
+    admit. (* TODO: are these two axioms?? *)
+    inv H. *)
+  - simpl in H.
+    (* rewrite multi'_iff_comp in H.
+    dependent induction H. *)
+    edestruct destr_app_compile; eauto.
+    destruct_conjs.
+    rewrite H4.
+    econstructor; eauto.
+    (*
+    
+    
+    + admit.
+    + admit.
+    + 
+      econstructor.
+      
+      eapply IHt1. 
+      Search (_ ++ _ = _ ++ _).
+      
+      
+
+
+
+
+
+
+
+
+    
+    inv H.
+    + congruence.
+    + 
+      
+    simpl in H1.
+    econstructor.
+    
+    edestruct destr_app_compile in H; eauto; destruct_conjs.
+    subst.
+    econstructor.
+    eapply IHt1; eauto.
+    + unfold not. intros.
+      subst.
+      inv H2.
+      ++ admit. (* TODO: compile not empty lemma *)
+      ++ dependent destruction x'.
+         inv H9.
+      * admit.
+      * admit.
+
+    
+    + eapply IHt2; eauto.
+      {
+      unfold not. intros.
+      subst.
+      inv H4.
+      * admit.
+      * admit. } *)
+  - simpl in H.
+    destruct s.
+    inv H.
+    inv H0.
+    inv H7. doit.
+    (*admit.
+    
+    inv H8. doit.
+
+    assert (
+        refl_trans_1n_trace vm_step'
+         {|
+         cec := e1;
+         cvm_list := instr_compiler t1 ++
+                     abesr :: instr_compiler t2 ++ [ajoins (Nat.pred (snd r))];
+         cvm_stack := e2 :: vm_stack r0 |}
+         {| cec := ec r'; cvm_list := []; cvm_stack := vm_stack r' |} cs'
+        =
+        vm_1n_multi' (mk_accum e1 (e2 :: vm_stack r0)) r'
+                     (instr_compiler t1 ++
+                                     abesr :: instr_compiler t2 ++ [ajoins (Nat.pred (snd r))])
+                     []
+                     cs').
+    auto.
+    rewrite H in H2. clear H.   *)                
+
+    edestruct destr_app_compile' in H1.
+        assert (
+        refl_trans_1n_trace vm_step'
+         {|
+         cec := e1;
+         cvm_list := instr_compiler t1 ++
+                     abesr :: instr_compiler t2 ++ [ajoins (Nat.pred (snd r))];
+         cvm_stack := e2 :: vm_stack r0 |}
+         {| cec := ec r'; cvm_list := []; cvm_stack := vm_stack r' |} cs'
+        =
+        vm_1n_multi' (mk_accum e1 (e2 :: vm_stack r0)) r'
+                     (instr_compiler t1 ++
+                                     abesr :: instr_compiler t2 ++ [ajoins (Nat.pred (snd r))])
+                     []
+                     cs').
+        auto.
+        rewrite <- H. eauto.
+        
+    destruct_conjs. doit.
+    assert (trace t1 x).
+    {
+      eapply IHt1.
+      eassumption.
+    }
+    clear H1.
+    inv H3. doit.
+    inv H1. doit.
+    inv H10. doit.
+
+    assert ( refl_trans_1n_trace vm_step'
+         {|
+         cec := er;
+         cvm_list := instr_compiler t2 ++ [ajoins (Nat.pred (snd r))];
+         cvm_stack := e :: vm_stack r'2 |}
+         {| cec := ec r'; cvm_list := []; cvm_stack := vm_stack r' |} cs'0
+             =
+             vm_1n_multi' (mk_accum er (e :: vm_stack r'2))
+                          r'
+                          (instr_compiler t2 ++ [ajoins (Nat.pred (snd r))])
+                          []
+                          cs'0).
+    auto.
+    rewrite H1 in H6. clear H1. doit.
+
+    edestruct destr_app_compile'' in H6; eauto.
+    destruct_conjs.
+    assert (trace t2 x0).
+    {
+      eapply IHt2; eauto.
+    }
+    rewrite H7.
+    inv H4. doit.
+    inv H9. doit. inv H14. doit. simpl in *.
+    dependent destruction H1. doit.
+    simpl in *.
+    assert (cs' = []).
+    {
+    inv H10.
+    + eauto.
+    + inv H1. }
+    rewrite H1.
+    econstructor; eauto. 
+  -
+Admitted.
+
+Theorem vm_ordered : forall t e e' s tr ev0 ev1,
+    well_formed t ->
+    vm_1n_multi'
+    (mk_accum e s) (mk_accum e' s)
+    (instr_compiler t) [] tr ->
+    prec (ev_sys t) ev0 ev1 ->
+    earlier tr ev0 ev1.
+Proof.
+  intros.
+  apply vm_lstar_trace in H0; auto.
+  apply trace_order with (t:=t); auto.
+  (*  
+  intros.
+  edestruct vm_smallstep with (p:=0); eauto.
+  eapply ordered; eauto. *)
+Defined.
 
 Lemma vm_config_correct : forall e s t tr,
     trace t tr ->
     vm_1n_multi (mk_vm_config e                  (instr_compiler t) s)
                 (mk_vm_config (eval (unanno t) e)[]                 s)
                 tr.
-Proof with doit.
+Proof.
   intros.
   generalize dependent e.
   generalize dependent s.
@@ -892,39 +1327,12 @@ Proof with doit.
   induction t; intros; simpl in *.
   - inv H.
     destruct a; eapply step_implies_lstar; econstructor.
-  - inv H.
-    (* assert  ((req (fst r) n (unanno t) :: tr1 ++ [rpy (Nat.pred (snd r)) n]) =
-             ((req (fst r) n (unanno t) :: tr1) ++ [rpy (Nat.pred (snd r)) n])).
-    simpl. eauto. *)
-    
+  - inv H. 
     eapply step_implies_lstar.
     rewrite <- remote_events_axiom with (t:=t) (tr:=tr1).
-
     eapply reqrpy_step. assumption.
   - inv H.
     eapply vm_1n_multi_trans with (y:=mk_vm_config (eval (unanno t1) e) (instr_compiler t2) s).
-    Lemma jj : forall e e' s t rest tr,
-      vm_1n_multi
-           {| cec := e; cvm_list := instr_compiler t; cvm_stack := s |}
-           {| cec := e'; cvm_list := []; cvm_stack := s |} tr ->
-
-      vm_1n_multi
-        {| cec := e;
-           cvm_list := instr_compiler t ++ rest ;
-           cvm_stack := s |}
-        {| cec := e';
-           cvm_list := rest;
-           cvm_stack := s |} tr.
-    Proof.
-      intros.
-      assert (rest = [] ++ rest). simpl. reflexivity.
-      rewrite H0 at 2.
-      assert (tr = tr ++ []). rewrite app_nil_r. auto.
-      rewrite H1.
-      eapply vm_1n_multi_transitive'. apply H.
-      simpl. econstructor.
-    Defined.
-
     apply jj; eauto.
     apply IHt2; eauto.
   - destruct s.
@@ -948,14 +1356,6 @@ Proof with doit.
     apply step_implies_lstar.
     econstructor.
   - destruct s.
-    (*assert ([asplit (fst r) s s1;
-                abep (range t1) (range t2) (instr_compiler t1)
-                     (instr_compiler t2); ajoinp (Nat.pred (snd r))] =
-            [asplit (fst r) s s1] ++ 
-                [abep (range t1) (range t2) (instr_compiler t1)
-                      (instr_compiler t2)] ++ [ajoinp (Nat.pred (snd r))]).
-    auto.
-    rewrite H0.*)
     inv H.
     assert ((Term.split (fst r) :: tr2 ++ [join (Nat.pred (snd r))]) =
             [(Term.split (fst r))] ++ tr2 ++ [join (Nat.pred (snd r))]). auto.
@@ -966,9 +1366,6 @@ Proof with doit.
     econstructor.
     econstructor.
     econstructor.
-    Axiom hihi : forall t tr,
-      trace t tr ->
-      parallel_vm_events (instr_compiler t) = tr.
 
     rewrite hihi with (t:=t1) (tr:=tr0).
     rewrite hihi with (t:=t2) (tr:=tr1).
@@ -982,410 +1379,51 @@ Proof with doit.
     econstructor.
 Defined.
 
-    
-    
-    
-  
 
-(*
-Lemma vm_config_correct : forall e e' s s' t tr,
-    vm_1n_multi (mk_vm_config e (instr_compiler t) s)
-                (mk_vm_config e'[]                 s')
+Lemma vm_config_deterministic : forall e e' e'' s s' s'' il il' tr tr',
+  vm_1n_multi (mk_vm_config e il s) (mk_vm_config e' il' s') tr ->
+  vm_1n_multi (mk_vm_config e il s) (mk_vm_config e'' il' s'') tr' ->
+  e' = e'' /\
+  s' = s''.
+Proof.
+Admitted.
+
+Lemma vm_config_correct' : forall e e' s s' t tr,
+    vm_1n_multi' (mk_accum e s) (mk_accum e' s')
+                 (instr_compiler t) []
                 tr ->
     e' = (eval (unanno t) e) /\
     s = s'.
-Proof with doit.
-  intros.
-  generalize dependent e.
-  generalize dependent e'.
-  generalize dependent s.
-  generalize dependent s'.
-  generalize dependent tr.
-  induction t; intros; simpl in *.
-  - destruct a.
-    + inv H. inv H0.
-    simpl.
-    inv H7.
-    inv H1.
-    split; reflexivity.
-    inv H.
-    + inv H. inv H0.
-    simpl.
-    inv H7.
-    inv H1.
-    split; reflexivity.
-    inv H.
-    + admit.
-    + admit.
-    + admit.
-  - inv H. inv H0. inv H7. inv H1. simpl.
-    split; reflexivity.
-    inv H.
-  - 
-    edestruct ffff with (r:=mk_accum e s) (r3:=mk_accum e' s'). unfold vm_1n_multi'. simpl. apply H.
-    destruct_conjs. unfold vm_1n_multi' in *.
-    doit.
-    dependent destruction x. doit.
-    edestruct IHt1; eauto.
-    doit.
-    edestruct IHt2; eauto.
-    split; simpl in *; congruence.
-  - destruct s. doit.
-    (*rewrite <- vm_n1_iff_1n in H.*)
-    inv H. doit. dependent destruction x'.
-
-
-    inv H0. doit. inv H9. doit.
-    edestruct ffff with (r:=mk_accum e1 (e2::s0)) (r3:=mk_accum e' s'). unfold vm_1n_multi'. apply H1.
-    destruct_conjs.
-    doit.
-    dependent destruction x. doit.
-    edestruct IHt1; eauto. doit.
-    rewrite <- H5 in H3.
-    rewrite H4 in H3.
-    
-    inv H3. doit.
-    dependent destruction x'. doit.
-    inv H6. doit. inv H12. doit.
-
-    
-    edestruct ffff with (r:=mk_accum er (e6::s0)) (r3:= mk_accum e' s').
-    apply H7. doit.
-    destruct_conjs. doit.
-    dependent destruction x. doit.
-    edestruct IHt2; eauto. doit.
-    inv H5. doit.
-    dependent destruction x'. doit.
-    inv H9. doit. inv H15. doit.
-    inv H10. split; eauto.
-    inv H4.
-  -
-Admitted.
-  *)
-
-
-
-
-
-(*
-Lemma vm_config_correct : forall e e' s s' t tr,
-    vm_lstar (mk_accum e s) (mk_accum e' s')
-             (instr_compiler t) []
-             tr ->
-    e' = (eval (unanno t) e) /\
-    s = s'.
 Proof.
   intros.
-  generalize dependent e.
-  generalize dependent e'.
-  generalize dependent s.
-  generalize dependent s'.
-  generalize dependent tr.
-  induction t; intros.
-  - destruct a; inv_vm_lstar; (split; auto).
-  - simpl.
-    inv H. inv H4.
-    inv H7.
-    split; eauto.
-  - simpl.
-    simpl in H.
-    apply ffff_gen in H.
-    destruct_conjs.
-    destruct H. 
-    edestruct IHt2. eassumption.
-    edestruct IHt1. eassumption.
-    subst. split; reflexivity.
-    apply compile_not_empty.
-  - simpl in H. destruct s.
-    invv.
-    apply ffff_gen in H7.
-    destruct_conjs.
-    dependent destruction r''.
-    dependent destruction H7.
-    destruct IHt1 with (tr:=H) (s:=e2 :: s0) (s':=vm_stack0) (e:=splitEv s e) (e':=ec0).
-    apply H0.                  
-    invv.
-    dependent destruction r'''.
-    invv.
-    apply ffff_gen in H12.
-    destruct_conjs.
-    dependent destruction H12.   
-    destruct IHt2 with (tr:=H1) (s:=e0 :: s0) (s':=vm_stack0) (e:=splitEv s1 e) (e':=ec0).
-    apply H2.
-    invv.
-    dependent destruction r''1.
-    invv.
-    inv H14.
-    invv.
-    split.
-    eapply ssc_inv.
-    eauto. eauto. reflexivity.
-    apply compile_not_empty.
-    apply compile_not_empty.
-  - simpl in H. destruct s.
-    invv.
-    dependent destruction r''.
-    inv H9.
-    split; eauto.
-    rewrite para_eval_vm.
-    rewrite para_eval_vm.
-    eauto.
-Defined. *)
-(*
-Lemma stack_restore_vm : forall e e' s s' t tr,
-    vm_lstar (mk_accum e s) (mk_accum e' s')
-             (instr_compiler t) [] tr ->
-    s = s'.
-Proof.
-  intros.
-  edestruct vm_config_correct; eauto.
-Defined.*)
+  assert (trace t tr).
+  eapply vm_lstar_trace.
+  Check vm_config_correct.
+  assert (vm_1n_multi
+         {| cec := e; cvm_list := instr_compiler t; cvm_stack := s |}
+         {| cec := eval (unanno t) e; cvm_list := []; cvm_stack := s |} tr).
+  apply vm_config_correct.
+  eapply vm_lstar_trace. eassumption.
+  eassumption.
 
-(*
-Lemma vm_ev_stack_deterministic : forall r r' r'' il il' tr tr',
-  vm_lstar r r' il il' tr ->
-  vm_lstar r r'' il il' tr' ->
-  vm_stack r' = vm_stack r'' /\
-  ec r' = ec r''.
-Proof.
-Admitted. *)
-
-Lemma destr_app_compile : forall r0 r' t1 t2 tr,
-    vm_1n_multi' r0 r' (instr_compiler t1 ++ instr_compiler t2) [] tr
-    -> (exists tr1 r_mid,
-          vm_1n_multi' r0 r_mid (instr_compiler t1) [] tr1 /\
-          exists tr2,
-            vm_1n_multi' r_mid r' (instr_compiler t2) [] tr2 /\
-            tr = tr1 ++ tr2).
-Proof.
-  intros.
-  
-Admitted.
-
-Lemma destr_app_compile': forall r0 r' t1 t2 tr n,
-    vm_1n_multi' r0 r' (instr_compiler t1 ++
-                         abesr :: instr_compiler t2 ++ [ajoins n]) [] tr
-    -> (exists tr1 r_mid,
-          vm_1n_multi' r0 r_mid (instr_compiler t1) [] tr1 /\
-          exists tr2,
-            vm_1n_multi' r_mid r' (abesr :: instr_compiler t2 ++ [ajoins n]) [] tr2 /\
-            tr = tr1 ++ tr2).
-Proof.
-  intros.
-Admitted.
-
-    Lemma destr_app_compile'': forall r0 r' t2 tr n,
-    vm_1n_multi' r0 r' (instr_compiler t2 ++ [ajoins n]) [] tr
-    -> (exists tr1 r_mid,
-          vm_1n_multi' r0 r_mid (instr_compiler t2) [] tr1 /\
-          exists tr2,
-            vm_1n_multi' r_mid r' ([ajoins n]) [] tr2 /\
-            tr = tr1 ++ tr2).
-    Proof.
-    Admitted.
-
-Lemma vm_lstar_trace: forall r r' t tr,
-    (*well_formed t -> *)
-    vm_1n_multi' r r'
-             (instr_compiler t) []
-             tr ->
-    trace t tr.
-Proof.
-  intros.
-  assert (tr <> []). admit.
-  generalize dependent r.
-  generalize dependent r'.
-  generalize dependent tr.
-  induction t; intros.
-  - destruct a; simpl.
-    + simpl.
-      inv H.
-      inv H1. inv H8.
-      inv H2.
-      * simpl. econstructor.
-      * inv H.
-    + simpl.
-      inv H.
-      inv H1. inv H8.
-      inv H2.
-      * simpl. econstructor.
-      * inv H.
-    + simpl.
-      inv H.
-      inv H1. inv H8.
-      inv H2.
-      * simpl. econstructor.
-      * inv H.
-    + simpl.
-      inv H.
-      inv H1. inv H8.
-      inv H2.
-      * simpl. econstructor.
-      * inv H.
-    + simpl.
-      inv H.
-      inv H1. inv H8.
-      inv H2.
-      * simpl. econstructor.
-      * inv H.
-  - inv H.
-    dependent destruction x'.
-    inv H1. inv H10.
-    inv H2.
-    simpl. rewrite app_nil_r.
-    
-    econstructor.
-    eapply IHt.
-    admit.
-    admit. (* TODO: are these two axioms?? *)
-    inv H.
-  - (*simpl in H. *)
-    edestruct destr_app_compile in H; eauto.
-    (*assert
-      (exists tr1 r_mid,
-          vm_1n_multi' r0 r_mid (instr_compiler t1) [] tr1 /\
-          exists tr2,
-            vm_1n_multi' r_mid r' (instr_compiler t2) [] tr2). 
-
-
-    eapply destr_app_compile; eauto. *)
-
-    destruct_conjs.
-    subst.
-    econstructor.
-    eapply IHt1.
-    unfold not. intros.
-    subst.
-    inv H2.
-    + admit. (* TODO: compile not empty lemma *)
-    + dependent destruction x'.
-      inv H9.
-      * admit.
-      * admit.
-
-    + eassumption.
-    + eapply IHt2.
-      unfold not. intros.
-      subst.
-      inv H4.
-      * admit.
-      * admit.
-      * eassumption.
-  - simpl in H.
-    destruct s.
-    inv H.
-    inv H1.
-    inv H8. doit.
-
-    assert (
-        refl_trans_1n_trace vm_step'
-         {|
-         cec := e1;
-         cvm_list := instr_compiler t1 ++
-                     abesr :: instr_compiler t2 ++ [ajoins (Nat.pred (snd r))];
-         cvm_stack := e2 :: vm_stack r0 |}
-         {| cec := ec r'; cvm_list := []; cvm_stack := vm_stack r' |} cs'
-        =
-        vm_1n_multi' (mk_accum e1 (e2 :: vm_stack r0)) r'
-                     (instr_compiler t1 ++
-                                     abesr :: instr_compiler t2 ++ [ajoins (Nat.pred (snd r))])
-                     []
-                     cs').
-    auto.
-    rewrite H in H2. clear H.                   
-
-    edestruct destr_app_compile' in H2; eauto. clear H2.
-    destruct_conjs. doit.
-    assert (trace t1 x).
-    eapply IHt1.
-    admit.
-    eassumption.
-    clear H1.
-    inv H3. doit.
-    inv H1. doit.
-    inv H10. doit.
-
-    assert ( refl_trans_1n_trace vm_step'
-         {|
-         cec := er;
-         cvm_list := instr_compiler t2 ++ [ajoins (Nat.pred (snd r))];
-         cvm_stack := e :: vm_stack r'2 |}
-         {| cec := ec r'; cvm_list := []; cvm_stack := vm_stack r' |} cs'0
-             =
-             vm_1n_multi' (mk_accum er (e :: vm_stack r'2))
-                          r'
-                          (instr_compiler t2 ++ [ajoins (Nat.pred (snd r))])
-                          []
-                          cs'0).
-    auto.
-    rewrite H1 in H6. clear H1.
-
-    edestruct destr_app_compile'' in H6; eauto.
-    destruct_conjs.
-    assert (trace t2 x0).
-    eapply IHt2; eauto.
-    admit.
-    rewrite H7.
-    inv H4. doit.
-    inv H9. doit. inv H14. doit. simpl in *.
-    dependent destruction H1. doit.
-    simpl in *.
-    assert (cs' = []).
-    inv H10.
-    + eauto.
-    + inv H1.
-    rewrite H1.
-    econstructor; eauto.
-  -
-    
-    
-    
-    rewrite <- vm_n1_iff_1n in H6.
-    inv H6.
-    admit.
-    
-    
-
-          
-      
-        
-      
-      
-      
-    
-      
-  -
-    
-      
-    
-    
-    + congruence.
-    + dependent destruction H1.
-      
-      
-    
-    
-
-
-  
-Admitted.
-
-Theorem vm_ordered : forall t e e' s tr ev0 ev1,
-    well_formed t ->
-    vm_lstar
-    (mk_accum e s) (mk_accum e' s)
-    (instr_compiler t) [] tr ->
-    prec (ev_sys t) ev0 ev1 ->
-    earlier tr ev0 ev1.
-Proof.
-  intros.
-  apply vm_lstar_trace in H0; auto.
-  apply trace_order with (t:=t); auto.
-  (*  
-  intros.
-  edestruct vm_smallstep with (p:=0); eauto.
-  eapply ordered; eauto. *)
+  assert (vm_1n_multi
+         {| cec := e; cvm_list := instr_compiler t; cvm_stack := s |}
+         {| cec := eval (unanno t) e; cvm_list := []; cvm_stack := s |} tr).
+  apply vm_config_correct; eauto.
+  unfold vm_1n_multi' in H. doit.
+  edestruct vm_config_deterministic.
+  apply H. apply H1.
+  split; auto.
 Defined.
+  
+
+
+
+
+
+
+
+
 
 
 
@@ -1617,3 +1655,29 @@ Proof.
   inv H.
   simpl. reflexivity.
 Defined. *)
+
+
+
+
+
+
+(* Alternate multistep relation:  
+
+Inductive vm_comp_multi : vm_accum -> vm_accum -> list AnnoInstr -> list AnnoInstr -> list Ev -> Prop :=
+| vm_lstar_refl: forall r l, vm_comp_multi r r l l []
+| vm_lstar_step: forall r r' i tr,
+    vm_step r i r' tr ->
+    vm_comp_multi r r' [i] [] tr
+| vm_lstar_comp: forall r r' r'' tr1 tr2 resl t1 t2 il1 il2,
+    il1 = instr_compiler t1 ->
+    il2 = instr_compiler t2 ->
+    vm_comp_multi r r' il1 [] tr1 ->
+    vm_comp_multi r' r'' il2 resl tr2 ->
+    vm_comp_multi r r'' (il1 ++ il2) resl (tr1 ++ tr2).
+
+Lemma multi'_iff_comp : forall r r' l l' tr,
+    vm_1n_multi' r r' l l' tr <-> vm_comp_multi r r' l l' tr.
+Proof.
+Admitted.
+
+*)
